examples/sbf/verif_Filter.v
@@ -23,3 +23,38 @@ Definition p := ["pipe"; "ingress"; "bf2_ds"].
 
 Definition Filter_fundef :=
   ltac:(get_fd ["Bf2BloomFilter"; "apply"] ge).
+
+Definition regact_clear_index_apply_fd :=
+  ltac:(get_am_fd ge am_ge (p ++ ["regact_clear_index"; "apply"]) ge).
+
+Definition regact_clear_index_apply_spec : func_spec :=
+  RegisterAction_apply_spec (p ++ ["regact_clear_index"]) (fun i => ValBaseBit (P4Arith.to_lbool 32 i))
+    (fun i => i + 1) (fun i => P4Bit 32 i).
+
+Lemma regact_clear_index_apply_body :
+  func_sound am_ge regact_clear_index_apply_fd nil regact_clear_index_apply_spec.
+Proof.
+  start_function.
+  step.
+  step.
+  step.
+  step.
+  entailer.
+  { red.
+    fold abs_plus.
+    unfold eval_p4int_sval.
+    cbn [width_signed].
+    change (eval_val_to_sval (ValBaseBit (P4Arith.to_lbool 32 old_value)))
+      with (ValBaseBit (P4Arith.to_loptbool 32 old_value)).
+    rewrite abs_plus_bit.
+    apply sval_refine_refl.
+  }
+Qed.
+
+Definition regact_clear_index_execute_body :=
+  ltac:(build_execute_body ge regact_clear_index_apply_body).
+
+#[local] Hint Extern 5 (func_modifies _ _ _ _ _) => (apply regact_clear_index_execute_body) : func_specs.
+
+Definition act_clear_index_fd :=
+  ltac:(get_fd ["Bf2BloomFilter"; "act_clear_index"] ge).
